Update sexpr representation to have typesafe atoms.

lean/deps/typed_smt2/src/galois/sexpr.lean
@@ -3,8 +3,26 @@ This declares an s-expression datatype for generating
 expressions and reasoning about their interpretation.
 -/
 import system.io
-import galois.data.buffer
+import data.array.lemmas -- from mathlib
 
+import galois.data.array
+import galois.data.buffer
+import galois.data.list
+import galois.data.nat
+
+import .char_reader
+
+meta def dec_trivial_tac : tactic unit := do
+  tgt ← tactic.target,
+  let e := (`(@of_as_true) : expr) tgt,
+  r ← tactic.apply e,
+  tactic.exact `(trivial)
+
+universes u v w
+
+/--
+Meta class for compile-time parsing of strings to data types.
+-/
 meta class is_meta_string (α : Type) :=
 (parse : string → except string α)
 (to_expr {} : α → tactic expr)
@@ -21,34 +39,196 @@ meta def coerce (s:string) (α:Type) [is_meta_string α]  : tactic unit := do
 
 namespace sexpr
 
+namespace atom
+
+/-- Recognize legal characters in s-expressions. -/
+def is_legal_char (c:char) : Prop := not (c ∈ ['(', ')', ' ', '\t', '\n'])
+
+instance is_legal_char.decidable : decidable_pred is_legal_char :=
+begin
+  intro c,
+  unfold atom.is_legal_char,
+  apply_instance
+end
+
+theorem is_legal_digit_char (n:ℕ) : is_legal_char (nat.digit_char n) :=
+begin
+  unfold nat.digit_char,
+  by_cases (n =  0); simp only [h,if_pos, if_false], {dec_trivial_tac,},
+  by_cases (n =  1); simp only [h,if_pos, if_false], {dec_trivial_tac,},
+  by_cases (n =  2); simp only [h,if_pos, if_false], {dec_trivial_tac,},
+  by_cases (n =  3); simp only [h,if_pos, if_false], {dec_trivial_tac,},
+  by_cases (n =  4); simp only [h,if_pos, if_false], {dec_trivial_tac,},
+  by_cases (n =  5); simp only [h,if_pos, if_false], {dec_trivial_tac,},
+  by_cases (n =  6); simp only [h,if_pos, if_false], {dec_trivial_tac,},
+  by_cases (n =  7); simp only [h,if_pos, if_false], {dec_trivial_tac,},
+  by_cases (n =  8); simp only [h,if_pos, if_false], {dec_trivial_tac,},
+  by_cases (n =  9); simp only [h,if_pos, if_false], {dec_trivial_tac,},
+  by_cases (n = 10); simp only [h,if_pos, if_false], {dec_trivial_tac,},
+  by_cases (n = 11); simp only [h,if_pos, if_false], {dec_trivial_tac,},
+  by_cases (n = 12); simp only [h,if_pos, if_false], {dec_trivial_tac,},
+  by_cases (n = 13); simp only [h,if_pos, if_false], {dec_trivial_tac,},
+  by_cases (n = 14); simp only [h,if_pos, if_false], {dec_trivial_tac,},
+  by_cases (n = 15); simp only [h,if_pos, if_false], {dec_trivial_tac,},
+  dec_trivial_tac,
+end
+
+/-- Indicate if all characters in buffer are well-formed. -/
+def well_formed (b:char_buffer) : Prop
+  := ∀i, atom.is_legal_char (b.read i)
+  ∧ b ≠ buffer.nil
+
+namespace well_formed
+
+local attribute [reducible] well_formed
+instance decidable : decidable_pred well_formed := by apply_instance
+
+end well_formed
+end atom
+
+/-- This denotes an atom in the s-expression syntax.
+
+We have not done this yet, but we will need to adds
+-/
 structure atom :=
 (to_char_buffer : char_buffer)
+(valid : atom.well_formed to_char_buffer)
 
 namespace atom
 
+protected def to_repr (a:atom) : string := a.to_char_buffer.to_string
+
+instance : has_repr atom := { repr := atom.to_repr }
+
 instance : decidable_eq atom := by tactic.mk_dec_eq_instance
+
+protected def lt (x y : atom) : Prop := x.to_char_buffer.to_string < y.to_char_buffer.to_string
+
+instance has_lt : has_lt atom := { lt := atom.lt }
+
+instance has_decidable_lt (x y : atom) : decidable (x < y) :=
+begin
+  simp [has_lt.lt, atom.lt],
+  apply_instance
+end
+
+/-- Map an s-expression to a meta-level expression -/
+protected
+meta def to_expr (c:atom) : tactic expr := do
+  let s := reflected.to_expr (string.reflect c.to_char_buffer.to_string),
+  let b := `(string.to_char_buffer %%s),
+  gs ← tactic.get_goals,
+  proof_var ← tactic.mk_meta_var `(atom.well_formed %%b),
+  tactic.set_goals [proof_var],
+  tgt ← tactic.target,
+  tactic.apply `(@of_as_true %%tgt),
+  success ← tactic.try_core (tactic.exact `(trivial)),
+  tactic.set_goals gs,
+  match success with
+  | option.none := tactic.fail $ repr c ++ " is an invalid s-expr atom."
+  | (option.some _):= do
+    pure `({ atom . to_char_buffer := %%b, valid := %%proof_var })
+  end
+
+@[simp]
+theorem size_push_back {α} (b:buffer α) (c:α)
+: (buffer.push_back b c).size = b.size + 1 :=
+begin
+  cases b,
+  trivial,
+end
+
+@[simp]
+theorem size_append_list {α} (b:buffer α) (l:list α)
+: (buffer.append_list b l).size = l.length + b.size :=
+begin
+  revert b,
+  induction l,
+  case list.nil {
+    intro b,
+    simp [buffer.append_list, nat.zero_add],
+  },
+  case list.cons : x r ind {
+    intro b,
+    simp only [buffer.append_list, ind, size_push_back, list.length_cons,
+               nat.add_succ, nat.add_zero, nat.succ_add],
+  },
+end
+
+theorem read_append_list_bound {α} {i:ℕ} {b:buffer α} {l:list α}
+: not (i < b.size)
+→ i < (buffer.append_list b l).size
+→ i - b.size < l.length :=
+begin
+  intros i_not_lt i_lt_append,
+  simp at i_not_lt,
+  simp only [size_append_list] at i_lt_append,
+  simp only [nat.sub_lt_to_add, i_lt_append, i_not_lt],
+  dec_trivial_tac,
+end
+
+/--
+This converts a nat to a char_buffer in decimal notation.
+
+Note. nat.repr seems to be builtin to the Lean VM magic, so it
+is much faster to invoke directly rather than using the functions
+used to define it.
+-/
+protected def nat_to_decimal_buffer (n : ℕ) : char_buffer :=
+  n.repr.to_char_buffer
+
+
+/-- Show that decimal numbers will be well-formed atoms. -/
+theorem nat_to_decimal_buffer_is_well_formed (x:ℕ) : atom.well_formed (atom.nat_to_decimal_buffer x) :=
+begin
+  unfold atom.well_formed,
+
+  intro i_fin,
+  cases i_fin with i i_lt,
+  dsimp only [atom.nat_to_decimal_buffer],
+  dsimp only [nat.repr],
+  simp only [buffer.read_to_nth_le],
+  simp only [buffer.to_char_buffer_as_string],
+  apply and.intro,
+  -- Show repr only returns valid characters.
+  { simp only [buffer.to_list_to_buffer],
+    simp only [list.nth_le_reverse_simp],
+    simp only [list.nth_le_map'],
+    apply is_legal_digit_char
+  },
+  -- Show repr is non-empty
+  { apply mt (congr_arg buffer.to_list),
+    -- For some reason, the simplification rules below require ne is explicitly used
+    apply ne.elim,
+    simp only [buffer.to_list_to_buffer, buffer.nil_to_list],
+    -- The other rules work better with the ne eliminated.
+    simp only [ne, list.reverse_eq_nil],
+    simp only [list.map_eq_nil],
+    apply nat.to_digits_ne_nil,
+  },
+end
+
+/- Construct a atom from the decimal notation of a nat. -/
+def nat_to_decimal (x:ℕ) : atom := ⟨atom.nat_to_decimal_buffer x, atom.nat_to_decimal_buffer_is_well_formed x⟩
 
 end atom
 
 /--
-This is a data-structure for representing non-empty
+This is a data-structure for representing non-empty lists of
+well-formed s-expressions.  It does not allow dotted lists directly,
+and they would instead be parsed as a list with a dot followed by
+an atom.
 
-The internal types are strictly general than what one may ordinarily
-expect of s-expressions to allow arbitrary strings to be converted into
-s-expressions, and concatenating two s-expressions.
-
-We do add a decidable_eq instance for s-expressions, but it is structural
-and two s expressions may be distinct, but render to the same string.
-The intent is to allow one to efficiently generate s-expressions,
-do lightweight pattern matching on them, and write them to handles.
+The term is structured to both simplify serialization and
+top-down/left-to-right parsing.
 -/
 inductive sexpr_list : Type
 | atom : atom → sexpr_list
-| empty_parens : sexpr_list
+| nil  : sexpr_list
 | parens : sexpr_list → sexpr_list
--- This appends two s-expressions with a space in between.
 | prepend_atom : atom → sexpr_list → sexpr_list
-| prepend_empty_parens : sexpr_list → sexpr_list
+| prepend_nil : sexpr_list → sexpr_list
+-- @prepend_parens x y@ denotes @(x) y@.
 | prepend_parens : sexpr_list → sexpr_list → sexpr_list
 
 namespace sexpr_list
@@ -56,25 +236,24 @@ namespace sexpr_list
 protected
 def render {α} [has_append α] (rend : char_buffer → α) : sexpr_list → α
 | (atom b) := rend b.to_char_buffer
-| empty_parens := rend "()".to_char_buffer
+| nil := rend "()".to_char_buffer
 | (parens s) := rend "(".to_char_buffer ++ (s.render ++ rend ")".to_char_buffer)
 | (prepend_atom b s) := rend b.to_char_buffer ++ (rend " ".to_char_buffer ++ s.render)
-| (prepend_empty_parens s) := rend "() ".to_char_buffer ++ s.render
+| (prepend_nil s) := rend "() ".to_char_buffer ++ s.render
 | (prepend_parens p s) :=
   rend "(".to_char_buffer ++ (p.render ++ (rend ") ".to_char_buffer ++ s.render))
 
 protected
 def to_repr (l:sexpr_list) : string := (sexpr_list.render id l).to_string
 
-
 /-- Return true if this is a single s-expression -/
 protected
 def is_single : sexpr_list → Prop
 | (atom _) := true
-| empty_parens := true
+| nil := true
 | (parens _) := true
 | (prepend_atom _ _) := false
-| (prepend_empty_parens _) := false
+| (prepend_nil _) := false
 | (prepend_parens _ _) := false
 
 instance (e:sexpr_list) : decidable (e.is_single) :=
@@ -85,26 +264,25 @@ end
 /-- Map an s-expression to a meta-level expression -/
 protected
 meta def to_expr : sexpr_list → tactic expr
-| (sexpr_list.atom ⟨c⟩) := do
-  let s := reflected.to_expr (string.reflect c.to_string) in
-  pure `(atom ⟨string.to_char_buffer %%s⟩)
-| empty_parens := do
-  pure `(empty_parens)
+| (sexpr_list.atom a) := do
+  ae ← a.to_expr,
+  pure `(atom %%ae)
+| nil := do
+  pure `(nil)
 | (parens s) := do
   e ← to_expr s,
   pure `(parens %%e)
-| (prepend_atom ⟨c⟩ y) := do
-  let s := reflected.to_expr (string.reflect c.to_string),
+| (prepend_atom a y) := do
+  ae ← a.to_expr,
   e ← to_expr y,
-  pure `(prepend_atom ⟨string.to_char_buffer %%s⟩ %%e)
-| (prepend_empty_parens y) := do
+  pure `(prepend_atom %%ae %%e)
+| (prepend_nil y) := do
   e ← to_expr y,
-  pure `(prepend_empty_parens %%e)
+  pure `(prepend_nil %%e)
 | (prepend_parens x y) := do
   xe ← to_expr x,
   ye ← to_expr y,
   pure `(prepend_parens %%xe %%ye)
-
 
 instance : decidable_eq sexpr_list := by tactic.mk_dec_eq_instance
 
@@ -134,7 +312,7 @@ protected
 def mk_atom (c:atom) : sexpr := ⟨sexpr_list.atom c, by {unfold sexpr_list.is_single}⟩
 
 protected
-def empty_parens : sexpr := ⟨sexpr_list.empty_parens, by {unfold sexpr_list.is_single}⟩
+def nil : sexpr := ⟨sexpr_list.nil, by {unfold sexpr_list.is_single}⟩
 
 protected
 def parens (c:sexpr_list) : sexpr := ⟨sexpr_list.parens c, by {unfold sexpr_list.is_single}⟩
@@ -144,7 +322,7 @@ namespace sexpr_list
 /-- Prepend sexpression to list -/
 def prepend : sexpr → sexpr_list → sexpr_list
 | ⟨sexpr_list.atom c, _⟩ y := prepend_atom c y
-| ⟨sexpr_list.empty_parens,_⟩ y := prepend_empty_parens y
+| ⟨sexpr_list.nil,_⟩ y := prepend_nil y
 | ⟨sexpr_list.parens x, _⟩ y := prepend_parens x y
 
 end sexpr_list
@@ -165,30 +343,16 @@ def of_list_core : sexpr → list sexpr → sexpr_list
 /-- Construct an s-expression from a list -/
 protected
 def of_list : list sexpr → sexpr
-| [] := sexpr.empty_parens
+| [] := sexpr.nil
 | (h::r) := sexpr.parens (sexpr.of_list_core h r)
 
-/-- A token read up so far -/
-structure partial_token :=
-(reversed_chars : list char)
+def read_atom {m} [char_reader string m] (n:ℕ) (b:char_buffer) : m atom := do
+  b1 ← char_reader.read_append_while atom.is_legal_char n b,
+  if h : atom.well_formed b1 then
+    pure ⟨b1, h⟩
+  else
+    throw $ repr b ++ " is not a valid atom."
 
-namespace partial_token
-
-/-- Create empty partial token -/
-def nil : partial_token := {reversed_chars := []}
-
-/-- Check if partial token is empty -/
-def empty (t:partial_token) : bool := t.reversed_chars.empty
-
-/-- Append a character to the end of a partial token -/
-def append (t:partial_token) (c:char) : partial_token :=
-  { reversed_chars := c :: t.reversed_chars }
-
-/-- Generate an s-expression from a partial token. -/
-def to_sexpr (t:partial_token) : sexpr :=
-  sexpr.mk_atom ⟨t.reversed_chars.reverse.as_string.to_char_buffer⟩
-
-end partial_token
 
 /-- A frame represents the first part of an s-expression that started with a open-paren -/
 structure frame :=
@@ -199,117 +363,90 @@ namespace frame
 /-- Create an empty frame -/
 def nil : frame := ⟨[]⟩
 
-/-- This adds the partial token as an sexpression if the token is non-empty -/
-def append_partial (f:frame) (t:partial_token) : frame :=
-  if t.empty then
-    f
-  else
-    ⟨t.to_sexpr :: f.exprs⟩
-
 /-- Close a frame by appending close paren -/
 def close : frame → sexpr
-| ⟨[]⟩ := sexpr.empty_parens
+| ⟨[]⟩ := sexpr.nil
 | ⟨h::r⟩ := sexpr.parens (list.foldl (λx y, prepend y x) h.val r)
+
+/-- This adds the partial token as an sexpression if the token is non-empty -/
+def append_sexpr (f:frame) (t:sexpr) : frame := ⟨ t :: f.exprs⟩
 
 /-- This adds the partial token as an sexpression if the token is non-empty -/
 def append_frame (f:frame) (t:frame) : frame := ⟨ t.close :: f.exprs⟩
 
---| frame.empty := parens sexpr.empty
---| (frame.non_empty s) := parens s
-
 end frame
 
-/-- Read to newline -/
-def read_to_newline {m} [monad m] [monad_except string m] (get_char : m char) : ℕ → m unit
-| nat.zero := throw "out of gas"
-| (nat.succ n) := do
-  c ← monad_lift get_char,
-  if c = '\n' then
-    pure ()
-  else if c.is_whitespace then
-    read_to_newline n
-  else
-    throw $ "Unexpected character at end of expression " ++ c.to_string
+
+section
+open char_reader
 
 /-- Read the s-expression from the handle/ -/
-def read_inner {m} [monad m] [monad_except string m] (get_char : m char)
-  : ℕ → partial_token → list frame → m sexpr
-| nat.zero prev frames := do
+def read_core {m} [char_reader string m]
+  : ℕ → list frame → m sexpr
+| nat.zero frames := do
   throw "out of gas"
-| (nat.succ n) prev frames := do
-  c ← monad_lift get_char,
-  if c = '(' then
-    match frames with
-    | [] :=
-      if prev.empty then
-        read_inner n partial_token.nil [frame.nil]
-      else
-        throw "Unexpected open paren"
-    | (top_frame::rest_frames) :=
-      read_inner n partial_token.nil (frame.nil :: top_frame.append_partial prev :: rest_frames)
-    end
-  else if c = ')' then
+| (nat.succ n) frames := do
+  mc ← peek_char,
+  match mc with
+  | option.none :=
+    throw "Unexpected end of expression."
+  | option.some '(' := do
+      consume_char *> read_core n (frame.nil :: frames)
+  | option.some ')' := do
     match frames with
     | [] :=
       throw "unexpected close paren"
-    | (top_frame::lower_frames) :=
-      let new_top := (top_frame.append_partial prev) in
+    | (top_frame::lower_frames) := do
+      consume_char,
       match lower_frames with
       | [] := do
-        read_to_newline get_char n,
-        pure new_top.close
+        pure top_frame.close
       | (return_frame::rest_frames) :=
-        read_inner n partial_token.nil (frame.append_frame return_frame new_top :: rest_frames)
+        read_core n (frame.append_frame return_frame top_frame :: rest_frames)
       end
     end
-  else if c = '\n' then
-    match frames with
-    | [] := do
-      pure prev.to_sexpr
-    | (top_frame::lower_frames) := do
-      throw "end of line reached before close paren"
-    end
-  else if c.is_whitespace then
-    match frames with
-    | [] := do
-      read_to_newline get_char n,
-      pure prev.to_sexpr
-    | (top_frame::lower_frames) := do
-      read_inner n partial_token.nil (top_frame.append_partial prev :: lower_frames)
-    end
-  else
-    read_inner n (prev.append c) frames
+  | option.some c :=
+    if c.is_whitespace then do
+      consume_char,
+      read_core n frames
+    else do
+      consume_char,
+      a ← sexpr.mk_atom <$> read_atom n (buffer.nil.push_back c),
+      match frames with
+      | [] := pure a
+      | (top_frame::lower_frames) := do
+        read_core n (top_frame.append_sexpr a :: lower_frames)
+      end
+  end
 
 /-- Read the s-expression from the handle/ -/
-def read {m} [monad m] [monad_except string m] (get_char : m char) (gas : ℕ) : m sexpr := do
-  read_inner get_char gas partial_token.nil []
+def read {m} [char_reader string m] (gas : ℕ) : m sexpr := do
+  read_core gas []
+
+end
+
+local attribute [instance] handle_char_reader.string_is_char_reader
 
 /-- Read the s-expression from the handle/ -/
 def read_from_handle (h:io.handle) : io (except string sexpr) := do
-  let get_char : except_t string io char := monad_lift $ io.fs.get_char h in
-  (read get_char (2^64-1)).run
+  let gas : ℕ := 2^64-1 in
+  handle_char_reader.read_to_newline h (sexpr.read gas)
+
+local attribute [instance] string_char_reader.string_is_char_reader
 
 def parse (s:string) : except string sexpr :=
-  let get_char : except_t string (state (list char)) char := do
-        s <- get,
-        match s with
-        | [] := throw "Unexpected end of string"
-        | (h::r) := do put r, pure h
-        end in
-  match (read get_char (s.length+2)).run.run (s.to_list ++ ['\n']) with
-  | ⟨r, _⟩ := r
-  end
+  let gas : ℕ := 2^64-1 in
+  string_char_reader.read_to_end s (sexpr.read gas)
 
 meta def to_expr : sexpr → tactic expr
-| ⟨sexpr_list.atom ⟨b⟩,_⟩ := do
-  let s := reflected.to_expr (string.reflect b.to_string) in
-  pure `(sexpr.mk_atom ⟨string.to_char_buffer %%s⟩)
-| ⟨empty_parens,_⟩ := do
-  pure `(sexpr.empty_parens)
+| ⟨sexpr_list.atom a,_⟩ := do
+   ae <- a.to_expr,
+   pure `(sexpr.mk_atom %%ae)
+| ⟨nil,_⟩ := do
+  pure `(sexpr.nil)
 | ⟨parens s, _⟩ := do
   e ← s.to_expr,
   pure `(sexpr.parens %%e)
-
 
 meta instance : is_meta_string sexpr :=
 { parse := sexpr.parse
@@ -329,7 +466,7 @@ def app (op:sexpr) (args : list sexpr) : sexpr := sexpr.parens (sexpr.of_list_co
 def bin_app (op:sexpr) (x y : sexpr) : sexpr :=
   sexpr.parens (prepend op (prepend x y.val))
 
-def from_nat (x:ℕ) : sexpr := sexpr.mk_atom ⟨x.repr.to_char_buffer⟩
+def from_nat (n:ℕ) : sexpr := sexpr.mk_atom (atom.nat_to_decimal n)
 
 instance : decidable_eq sexpr := by tactic.mk_dec_eq_instance
 
