lean/deps/galois_stdlib/src/galois/data/array.lean
@@ -1,0 +1,9 @@
+
+
+namespace array
+
+/-- Empty buffer converted to array is same as array.nil -/
+@[simp]
+theorem to_list_nil {α} : to_list (@nil α) = [] := eq.refl _
+
+end array
