lean/deps/galois_stdlib/src/galois/data/buffer.lean
@@ -1,10 +1,51 @@
 /-
 Provides a decidable_eq instance for buffer.
 -/
-import data.buffer
+import data.buffer.basic -- from mathlib
+
+import galois.data.array
 
 namespace buffer
 
-instance {α} [decidable_eq α] : decidable_eq (buffer α) := by tactic.mk_dec_eq_instance
+theorem to_list_length {α} (b: buffer α)
+: list.length (buffer.to_list b) = b.size :=
+begin
+  simp only [buffer.to_list, size, array.to_list_length],
+end
+
+/-- Replace nil.to_list with empty list. -/
+@[simp]
+theorem nil_to_list (α:Type _) : (@buffer.nil α).to_list = [] := refl []
+
+/-- Convert read to list read so we can use list lemmas -/
+theorem read_to_nth_le {α} (b: buffer α) (i:fin b.size)
+: buffer.read b i = list.nth_le b.to_list i.val ((to_list_length b).symm ▸ i.is_lt) :=
+begin
+  cases b with n a,
+  simp only [read, to_list, array.to_list_nth_le', to_array],
+end
+
+
+/-- Empty buffer converted to array is same as array.nil -/
+@[simp]
+theorem to_array_mk_buffer {α} : to_array mk_buffer = @array.nil α :=
+begin
+  apply array.ext,
+  intro i,
+  have h : false := fin.elim0 i,
+  contradiction,
+end
+
+/-- Converting list to bufer and back is round trip. -/
+theorem to_list_to_buffer {α} (l:list α) : l.to_buffer.to_list = l :=
+begin
+  unfold list.to_buffer,
+  simp only [to_list_append_list],
+  simp only [to_list, to_array_mk_buffer, array.to_list_nil, list.nil_append],
+end
+
+/- Simplify functions calling through as_string -/
+theorem to_char_buffer_as_string (l:list char)
+: l.as_string.to_char_buffer = l.to_buffer := eq.refl l.to_buffer
 
 end buffer
