lean_deps/galois_stdlib/src/galois/category/except.lean
@@ -1,0 +1,23 @@
+/-
+This provides a few missing definitions to the except monad
+-/
+
+namespace except
+section
+  universes u v
+  parameter {ε : Type u}
+
+  protected def catch {α : Type v} (ma : except ε α) (f : ε → except ε α) : except ε α :=
+  match ma with
+  | (except.error err) := f err
+  | (except.ok v) := except.ok v
+  end
+
+  protected def throw {α : Type v} :  ε → except ε α := except.error
+
+  instance : monad_except ε (except ε) :=
+  { throw := @except.throw
+  , catch := @except.catch
+  }
+end
+end except
